.

theories/Data/BinTree.v
@@ -1,11 +1,102 @@
+Require Import Coq.Arith.PeanoNat.
+Require Import Coq.Lists.List.
 Require Import DschingisKhan.Prelude.PreludeInit.
 Require Import DschingisKhan.Prelude.PreludeUtil.
 
 Module BinaryTree.
 
+  Import ListNotations.
+
   Inductive bintree (A : Type) : Type :=
   | BTnull : bintree A
   | BTnode (t_l : bintree A) (x : A) (t_r : bintree A) : bintree A
   .
+
+  Global Arguments BTnull {A}.
+  Global Arguments BTnode {A} (t_l) (x) (t_r).
+
+  Section ACCESSORIES.
+
+  Context {A : Type}.
+
+  Local Notation bintree := (bintree A).
+
+  Fixpoint getHeight (t : bintree) {struct t} : nat :=
+    match t with
+    | BTnull => 0
+    | BTnode t_l x t_r => 1 + max (getHeight t_l) (getHeight t_r)
+    end
+  .
+
+  Section QUEUE_SEARCH.
+
+  Fixpoint rk_bt (t : bintree) {struct t} : nat :=
+    match t with
+    | BTnull => 1
+    | BTnode t_l x t_r => 1 + rk_bt t_l + rk_bt t_r
+    end
+  .
+
+  Definition rk_queue (ts : list bintree) : nat :=
+    list_sum (map rk_bt ts)
+  .
+
+  Inductive bfs_spec : list bintree -> list A -> Prop :=
+  | bfs_nil
+    : bfs_spec [] []
+  | bfs_cons_null (ts : list bintree) (xs : list A)
+    (IH_SPEC : bfs_spec ts xs)
+    : bfs_spec (BTnull :: ts) xs
+  | bfs_cons_node (t_l : bintree) (x : A) (t_r : bintree) (ts : list bintree) (xs : list A)
+    (IH_SPEC : bfs_spec ([t_l; t_r] ++ ts) xs)
+    : bfs_spec (BTnode t_l x t_r :: ts) (x :: xs)
+  .
+
+  Definition bfs_withSpec (ts : list bintree)
+    : {xs : list A | forall xs' : list A, bfs_spec ts xs' <-> xs = xs'}.
+  Proof.
+    assert (RECURSOR : forall ts : list bintree, Acc (fun lhs : list bintree => fun rhs : list bintree => rk_queue lhs < rk_queue rhs) ts).
+    { exact (well_founded_relation_on_image rk_queue Nat.lt (@lt_strong_ind (@Acc nat lt) (@Acc_intro nat lt))). }
+    induction (RECURSOR ts) as [ts H_acc_inv IH]. clear H_acc_inv RECURSOR. destruct ts as [ | [ | t_l x t_r]].
+    - exists ([]). intros xs'. split.
+      + intros SPEC. inversion SPEC; subst. reflexivity.
+      + intros ?; subst xs'. econstructor 1.
+    - assert (IH_rk : rk_queue ts < rk_queue (BTnull :: ts)).
+      { cbn. eapply le_intro_S_n_le_S_m. reflexivity. }
+      pose proof (IH ts IH_rk) as [xs IH_bfs].
+      exists (xs). intros xs'. split.
+      + intros SPEC. inversion SPEC; subst. eapply IH_bfs. exact (IH_SPEC).
+      + intros ?; subst xs'. econstructor 2. eapply IH_bfs. reflexivity.
+    - assert (IH_rk : rk_queue ([t_l; t_r] ++ ts) < rk_queue (BTnode t_l x t_r :: ts)).
+      { cbn. eapply le_intro_S_n_le_S_m. rewrite Nat.add_assoc. reflexivity. }
+      pose proof (IH ([t_l; t_r] ++ ts) IH_rk) as [xs IH_bfs].
+      exists (x :: xs). intros xs'. split.
+      + intros SPEC. inversion SPEC; subst. eapply eq_congruence. eapply IH_bfs. exact (IH_SPEC).
+      + intros ?; subst xs'. econstructor 3. eapply IH_bfs. reflexivity.
+  Defined.
+
+  Definition bfs (ts : list bintree) : list A :=
+    proj1_sig (bfs_withSpec ts)
+  .
+
+  Lemma bfs_spec_iff (ts : list bintree) (xs : list A)
+    : bfs_spec ts xs <-> bfs ts = xs.
+  Proof. revert xs. exact (proj2_sig (bfs_withSpec ts)). Qed.
+
+  Theorem bfs_unfold (ts : list bintree) :
+    bfs ts =
+    match ts with
+    | [] => []
+    | BTnull :: ts' => bfs ts'
+    | BTnode t_l x t_r :: ts' => x :: bfs ([t_l; t_r] ++ ts')
+    end.
+  Proof.
+    destruct ts as [ | [ | t_l x t_r] ts']; eapply bfs_spec_iff; econstructor.
+    all: eapply bfs_spec_iff; reflexivity.
+  Qed.
+
+  End QUEUE_SEARCH.
+
+  End ACCESSORIES.
 
 End BinaryTree.
